Veritas.EAC.fst
@@ -1,151 +1,10 @@
 module Veritas.EAC
 
-open FStar.Seq
-open Veritas.Hash
-open Veritas.Interleave
-open Veritas.Key
-open Veritas.MultiSetHash
-open Veritas.Record
-open Veritas.SeqAux
-open Veritas.SeqMachine
-open Veritas.State
 open Veritas.StateSeqMachine
-open Veritas.Verifier
+module S = Veritas.State
 
 //Allow the solver to unroll recursive functions at most once (fuel)
 #push-options "--max_fuel 1 --max_ifuel 1 --initial_fuel 1 --initial_ifuel 1"
-
-type evict_vlog_entry = e:vlog_entry {is_evict e}
-type nevict_vlog_entry = e:vlog_entry {not (is_evict e)}
-
-type vlog_entry_ext =
-  | NEvict: e:vlog_entry{not (is_evict e)} -> vlog_entry_ext
-  | EvictMerkle: e:vlog_entry{is_evict_to_merkle e} -> v:value -> vlog_entry_ext
-  | EvictBlum: e:vlog_entry{is_evict_to_blum e} -> v:value -> tid:nat -> vlog_entry_ext
-
-type vlog_ext = seq (vlog_entry_ext)
-
-type eac_state =
-  | EACFail: eac_state
-  | EACInit: eac_state
-  | EACInStore: m:add_method -> v:value -> eac_state
-  | EACEvictedMerkle: v:value -> eac_state
-  | EACEvictedBlum: v:value -> t:timestamp -> j:nat -> eac_state
-
-let is_eac_state_evicted (s: eac_state): bool = 
-  match s with
-  | EACEvictedMerkle _ -> true
-  | EACEvictedBlum _ _ _ -> true
-  | _ -> false
-
-let eac_add (e: vlog_entry_ext) (s: eac_state) : eac_state =
-  match s with
-  | EACFail -> EACFail
-  | EACInit -> (
-    match e with
-    | NEvict (AddM (k,v) _) -> if v = init_value k then EACInStore MAdd v
-                               else EACFail
-    | _ -> EACFail
-    )
-
-  | EACInStore m v -> (
-    match e with
-    | NEvict (Get _ v') -> if (DVal v') = v then s
-                           else EACFail
-    | NEvict (Put _ v') -> if (DVal? v) then EACInStore m (DVal v')
-                           else EACFail
-    | EvictMerkle (EvictM _ _) v' -> if DVal? v && v' <> v then EACFail
-                               else EACEvictedMerkle v
-    | EvictBlum (EvictBM k k' t) v' j -> if DVal? v && v' <> v || m <> MAdd then EACFail
-                                  else EACEvictedBlum v t j
-    | EvictBlum (EvictB _ t) v' j ->  if DVal? v && v' <> v || m <> BAdd then EACFail
-                                else EACEvictedBlum v t j
-    | _ -> EACFail
-    )
-
-  | EACEvictedMerkle v -> (
-    match e with 
-    | NEvict (AddM (_,v') _) -> if v' = v then EACInStore MAdd v
-                                else EACFail
-    | _ -> EACFail
-  )
-
-  | EACEvictedBlum v t tid -> (
-    match e with
-    | NEvict (AddB (_,v') t' tid') -> if v' = v && t' = t && tid' = tid then EACInStore BAdd v
-                                else EACFail
-    | _ -> EACFail
-  )
-
-let eac_smk = SeqMachine EACInit EACFail eac_add
-
-let to_vlog_entry (ee:vlog_entry_ext): vlog_entry =
-  match ee with
-  | EvictMerkle e _ -> e
-  | EvictBlum e _ _ -> e
-  | NEvict e -> e
-
-let vlog_entry_ext_key (e: vlog_entry_ext): key =  
-  vlog_entry_key (to_vlog_entry e)
-  
-let eac_sm = PSM eac_smk vlog_entry_ext_key
-
-(* evict add consistency *)
-let eac (l:vlog_ext) = valid_all eac_sm l
-
-(* refinement of evict add consistent logs *)
-type eac_log = l:vlog_ext{eac l}
-
-let is_eac_log (l:vlog_ext): (r:bool{r <==> eac l}) = 
-  valid_all_comp eac_sm l
-
-let max_eac_prefix (l:vlog_ext{not (is_eac_log l)}): 
-  (i:nat{i < length l /\
-        is_eac_log (prefix l i) /\
-        not (is_eac_log (prefix l (i + 1)))}) =
-  max_valid_all_prefix eac_sm l
-                                       
-(* the state operations of a vlog *)
-let is_state_op (e: vlog_entry): bool =
-  match e with
-  | Get k v -> true
-  | Put k v -> true
-  | _ -> false
-
-(* map vlog entry to state op *)
-let to_state_op (e:vlog_entry {is_state_op e}): state_op =
-  match e with
-  | Get k v -> Veritas.State.Get k v
-  | Put k v -> Veritas.State.Put k v
-
-(* filter out the state ops of vlog *)
-let to_state_op_vlog (l: vlog) =
-  map to_state_op (filter_refine is_state_op l)
-
-(* valid eac states *)
-let valid_eac_state (st:eac_state): bool = st <> EACFail &&
-                                           st <> EACInit
-
-let is_evict_ext (e:vlog_entry_ext): bool = 
-  match e with
-  | EvictMerkle _ _ -> true
-  | EvictBlum _ _ _ -> true
-  | _ -> false 
-
-let value_ext (e:vlog_entry_ext{is_evict_ext e}): value = 
-  match e with
-  | EvictMerkle _ v -> v
-  | EvictBlum _ v _ -> v
-
-(* value of a valid state *)
-let value_of (st:eac_state {valid_eac_state st}): value =
-  match st with
-  | EACInStore _ v -> v
-  | EACEvictedMerkle v -> v
-  | EACEvictedBlum v _ _ -> v
-
-let to_vlog (l:vlog_ext) =
-  map to_vlog_entry l
 
 let lemma_comm_empty (le:vlog_ext{length le = 0}) (k:data_key):
   Lemma (to_state_op_vlog (to_vlog (partn eac_sm k le)) =
@@ -161,21 +20,21 @@ let lemma_comm_empty (le:vlog_ext{length le = 0}) (k:data_key):
 
   (* since le is empty, lek & lk = filter on k le is empty *)
   lemma_filter_empty (iskey vlog_entry_ext_key k);
-  assert(length lek = 0);
-  assert(length lk = 0);
+  //assert(length lek = 0);
+  //assert(length lk = 0);
 
   (* since lk is empty, lks is empty *)
   lemma_filter_empty is_state_op;
   lemma_empty lk;
-  assert(length lks = 0);
+  //assert(length lks = 0);
   lemma_empty lks;
 
-  assert(length l = 0);
+  //assert(length l = 0);
   lemma_empty l;
-  assert(length ls = 0);
+  //assert(length ls = 0);
   lemma_empty ls;
-  lemma_filter_empty (iskey key_of k);
-  assert(length lsk = 0);
+  lemma_filter_empty (iskey S.key_of k);
+  //assert(length lsk = 0);
   lemma_empty lsk
 
 let lemma_partn_state_append (le:vlog_ext{length le > 0}) (k:data_key):
@@ -198,23 +57,23 @@ let lemma_partn_state_append (le:vlog_ext{length le > 0}) (k:data_key):
   let ee = index le (n - 1) in
   let e = to_vlog_entry ee in
   let op = to_state_op e in
-  assert(is_state_op e);
-  assert(vlog_entry_ext_key ee = k);
+  //assert(is_state_op e);
+  //assert(vlog_entry_ext_key ee = k);
 
   lemma_filter_extend2 (iskey vlog_entry_ext_key k) le;
   lemma_prefix1_append lek' ee;
-  assert(lek = append1 lek' ee);
+  //assert(lek = append1 lek' ee);
 
   lemma_map_extend to_vlog_entry lek;
   lemma_prefix1_append lk' e;
-  assert(lk = append1 lk' e);
+  //assert(lk = append1 lk' e);
 
   lemma_filter_extend2 is_state_op lk;
   assert(equal lksr (append1 lksr' e));
   lemma_prefix1_append lksr' e;
 
   lemma_map_extend to_state_op lksr;
-  assert(lks = append1 lks' op);
+  //assert(lks = append1 lks' op);
   ()
 
 let lemma_partn_state_same (le:vlog_ext{length le > 0}) (k:data_key):
@@ -238,20 +97,20 @@ let lemma_partn_state_same (le:vlog_ext{length le > 0}) (k:data_key):
   let e = to_vlog_entry ee in
   if vlog_entry_ext_key ee <> k then (
     lemma_filter_extend1 (iskey vlog_entry_ext_key k) le;
-    assert(lek' = lek);
+    //assert(lek' = lek);
     ()
   )
   else (
     lemma_filter_extend2 (iskey vlog_entry_ext_key k) le;
     lemma_prefix1_append lek' ee;
-    assert(lek = append1 lek' ee);
+    //assert(lek = append1 lek' ee);
 
     lemma_map_extend to_vlog_entry lek;
     lemma_prefix1_append lk' e;
-    assert(lk = append1 lk' e);
+    //assert(lk = append1 lk' e);
 
     lemma_filter_extend1 is_state_op lk;
-    assert(lksr = lksr');
+    //assert(lksr = lksr');
     ()
   )
 
@@ -274,12 +133,12 @@ let lemma_state_partn_append (le:vlog_ext{length le > 0}) (k:data_key):
   let ee = index le (n - 1) in
   let e = to_vlog_entry ee in
   let op = to_state_op e in
-  assert(is_state_op e);
-  assert(vlog_entry_ext_key ee = k);
+  //assert(is_state_op e);
+  //assert(vlog_entry_ext_key ee = k);
 
   lemma_map_extend to_vlog_entry le;
   lemma_prefix1_append l' e;
-  assert(l = append1 l' e);
+  //assert(l = append1 l' e);
 
   lemma_filter_extend2 is_state_op l;
   assert(equal lsr (append1 lsr' e));
@@ -287,10 +146,10 @@ let lemma_state_partn_append (le:vlog_ext{length le > 0}) (k:data_key):
 
   lemma_map_extend to_state_op lsr;
   lemma_prefix1_append ls' op;
-  assert(ls = append1 ls' op);
+  //assert(ls = append1 ls' op);
 
-  lemma_filter_extend2 (iskey key_of k) ls;
-  assert(lsk = append1 lsk' op);
+  lemma_filter_extend2 (iskey S.key_of k) ls;
+  //assert(lsk = append1 lsk' op);
   ()
 
 let lemma_state_partn_same (le:vlog_ext{length le > 0}) (k:data_key):
@@ -313,11 +172,11 @@ let lemma_state_partn_same (le:vlog_ext{length le > 0}) (k:data_key):
 
   lemma_map_extend to_vlog_entry le;
   lemma_prefix1_append l' e;
-  assert(l = append1 l' e);
+  //assert(l = append1 l' e);
 
   if not (is_state_op e) then (
     lemma_filter_extend1 is_state_op l;
-    assert (lsr = lsr');
+    //assert (lsr = lsr');
     ()
   )
   else (
@@ -328,10 +187,10 @@ let lemma_state_partn_same (le:vlog_ext{length le > 0}) (k:data_key):
 
     lemma_map_extend to_state_op lsr;
     lemma_prefix1_append ls' op;
-    assert(ls = append1 ls' op);
+    //assert(ls = append1 ls' op);
 
-    lemma_filter_extend1 (iskey key_of k) ls;
-    assert(lsk = lsk');
+    lemma_filter_extend1 (iskey S.key_of k) ls;
+    //assert(lsk = lsk');
     ()
   )
 
@@ -360,25 +219,25 @@ let rec lemma_comm (le:vlog_ext) (k:data_key):
     let lsk' = partn ssm k ls' in
 
     lemma_comm le' k;
-    assert (lks' = lsk');
+    //assert (lks' = lsk');
 
     let ee = index le (n - 1) in
     let e = to_vlog_entry ee in
     if is_state_op e && vlog_entry_ext_key ee = k then (
       let op = to_state_op e in
       lemma_partn_state_append le k;
-      assert(lks = append1 lks' op);
+      //assert(lks = append1 lks' op);
 
       lemma_state_partn_append le k;
-      assert(lsk = append1 lsk' op);
+      //assert(lsk = append1 lsk' op);
       ()
     )
     else (
       lemma_partn_state_same le k;
-      assert(lks = lks');
+      //assert(lks = lks');
 
       lemma_state_partn_same le k;
-      assert(lsk = lsk');
+      //assert(lsk = lsk');
       ()
     )
   )
@@ -422,10 +281,10 @@ let lemma_value_type (le:vlog_ext {length le > 0}):
     lemma_valid_prefix eac_smk le 1;
     lemma_notempty_implies_noninit eac_smk (prefix le 1);
     let st1 = seq_machine_run eac_smk (prefix le 1) in
-    assert(valid_eac_state st1);
+    //assert(valid_eac_state st1);
 
     lemma_reduce_prefix EACInit eac_add le 1;
-    assert(st = reduce st1 eac_add (suffix le (n - 1)));
+    //assert(st = reduce st1 eac_add (suffix le (n - 1)));
 
     if DVal? (value_of st1) then
       lemma_reduce_property_closure eac_closure_pred1 st1 eac_add (suffix le (n - 1))
@@ -440,7 +299,7 @@ let lemma_first_entry_is_madd (le:vlog_ext):
   let st1 = seq_machine_run eac_smk le1 in
   lemma_valid_prefix eac_smk le 1;
   lemma_reduce_singleton EACInit eac_add le1;
-  assert(st1 = eac_add (index le 0) EACInit);
+  //assert(st1 = eac_add (index le 0) EACInit);
   ()
 
 let rec lemma_data_val_state_implies_last_put (le:vlog_ext):
@@ -456,7 +315,7 @@ let rec lemma_data_val_state_implies_last_put (le:vlog_ext):
   if n = 0 then (
     lemma_reduce_empty EACInit eac_add;
     lemma_empty le;
-    assert (EACInit = seq_machine_run eac_smk le);
+    //assert (EACInit = seq_machine_run eac_smk le);
     ()
   )
 
@@ -470,7 +329,7 @@ let rec lemma_data_val_state_implies_last_put (le:vlog_ext):
     )
     else match (index le 0) with
     | NEvict (AddM (k, v) _ ) ->
-      assert(value_of st = v);
+      //assert(value_of st = v);
       ()
   )
 
@@ -483,23 +342,23 @@ let rec lemma_data_val_state_implies_last_put (le:vlog_ext):
     // le and le' have the same value type
     lemma_value_type le;
     lemma_value_type le';
-    assert(DVal? (value_of (seq_machine_run eac_smk le')));
+    //assert(DVal? (value_of (seq_machine_run eac_smk le')));
 
     // induction
     lemma_data_val_state_implies_last_put le';
 
     // IH
     let st' = seq_machine_run eac_smk le' in
-    assert(DVal?.v (value_of st') = last_put_value_or_null (to_vlog le'));
+    //assert(DVal?.v (value_of st') = last_put_value_or_null (to_vlog le'));
 
     lemma_reduce_append2 EACInit eac_add le;
-    assert(st = eac_add (index le (n - 1)) st');
+    //assert(st = eac_add (index le (n - 1)) st');
 
     if Put? (to_vlog_entry (index le (n - 1))) then
       lemma_last_index_last_elem_sat Put? l
 
     else (
-      assert(value_of st' = value_of st);
+      //assert(value_of st' = value_of st);
       lemma_last_index_last_elem_nsat Put? l;
 
       if has_some_put l' then
@@ -530,22 +389,22 @@ let lemma_eac_k_implies_valid_get (le:vlog_ext) (i:seq_index le):
   let lei = prefix le i in
 
   lemma_first_entry_is_madd le;
-  assert(n > 1);
+  //assert(n > 1);
 
   lemma_get_implies_data_val_state le i;
-  assert(valid eac_smk lei);
-  assert(DVal? (value_of (seq_machine_run eac_smk lei)));
+  //assert(valid eac_smk lei);
+  //assert(DVal? (value_of (seq_machine_run eac_smk lei)));
 
   lemma_data_val_state_implies_last_put lei;
   let sti = seq_machine_run eac_smk lei in
-  assert(DVal? (value_of sti));
+  //assert(DVal? (value_of sti));
 
   let lei' = prefix le (i + 1) in
   lemma_valid_prefix eac_smk le (i + 1);
-  assert(EACFail <> (seq_machine_run eac_smk lei'));
+  //assert(EACFail <> (seq_machine_run eac_smk lei'));
 
   lemma_reduce_append2 EACInit eac_add lei';
-  assert(seq_machine_run eac_smk lei' = eac_add (index le i) sti);
+  //assert(seq_machine_run eac_smk lei' = eac_add (index le i) sti);
   ()
 
 let state_op_map (l:vlog) (i:seq_index (to_state_op_vlog l)):
@@ -566,7 +425,7 @@ let lemma_last_put_map (l:vlog):
   if has_some_put l then (
     let j = last_put_idx l in
     let i = filter_index_inv_map is_state_op l j in
-    assert(index ls i = to_state_op (index l j));
+    //assert(index ls i = to_state_op (index l j));
     lemma_last_index_correct2 Veritas.State.Put? ls i;
     let i' = last_put_idx_k ls in
     if i' = i then ()
@@ -594,11 +453,11 @@ let lemma_eac_k_implies_ssm_k_valid (le:eac_log) (k:data_key):
     let op = index lks i in
 
     lemma_first_invalid_implies_invalid_get (prefix lks (i + 1));
-    assert(Veritas.State.Get?.v op <> last_put_value_or_null_k (prefix lks i));
+    //assert(Veritas.State.Get?.v op <> last_put_value_or_null_k (prefix lks i));
 
     // index of entry in lk/lek that corresponds to i
     let j = (state_op_map lk i) in
-    assert(to_state_op(index lk j) = op);
+    //assert(to_state_op(index lk j) = op);
     lemma_eac_k_implies_valid_get lek j;
     lemma_map_prefix to_vlog_entry lek j;
     lemma_last_put_map (prefix lk j)
