Veritas.Verifier.Merkle.fst
@@ -92,10 +92,10 @@ let lemma_proving_ancestor_blum_bit (#p:pos) (itsl: eac_ts_log p) (k:key{k <> Ro
 let lemma_addm_ancestor_is_proving (#p:pos) (itsl: its_log p {length itsl > 0}):
   Lemma (requires (TL.is_eac_log (its_prefix itsl (length itsl - 1)) /\
                    AddM? (its_vlog_entry itsl (length itsl - 1))))
-        (ensures (Root <> vlog_entry_key (its_vlog_entry itsl (length itsl - 1)) /\        
+        (ensures (Root <> V.key_of (its_vlog_entry itsl (length itsl - 1)) /\        
                   AddM?.k' (its_vlog_entry itsl (length itsl - 1)) = 
                   proving_ancestor (its_prefix itsl (length itsl - 1))
-                                   (vlog_entry_key (its_vlog_entry itsl (length itsl - 1))))) = admit()
+                                   (V.key_of (its_vlog_entry itsl (length itsl - 1))))) = admit()
 
  let lemma_store_contains_proving_ancestor (#p:pos) (itsl: eac_ts_log p) 
   (tid:nat{tid < p}) (k:key{k <> Root}):
